bin/query/ExtractQuery.v
@@ -10,14 +10,14 @@ Require Import ExtrOcamlNativeString.
 Require Import ExtrOCamlInt63.
 Extraction Language OCaml.
 
-Require Import Games.Util.Show.
-Require Import Games.Util.IntHash.
-Require Import Games.Util.OMap.
+Require Import TBGen.Util.Show.
+Require Import TBGen.Util.IntHash.
+Require Import TBGen.Util.OMap.
 Require Import TBGen.Bear.Sort.
 Require Import TBGen.Bear.BearGame.
 Require Import TBGen.Bear.RomanWheel.
-Require Import Games.Game.TB.
-Require Import Games.Game.OCamlTB.
+Require Import TBGen.TB.TB.
+Require Import TBGen.TB.OCamlTB.
 
 Definition make_BG_State {G} (pl : Player.Player)
   (b h1 h2 h3 : Graph.Vert G) : option (BG_State G).
