theory/Util/NewLoop.v
@@ -1,0 +1,142 @@
+Require Import Lia.
+Require Import Compare_dec.
+
+
+Lemma iter_lemma {X} (f : X -> X) (k : nat) (x : X) :
+  Nat.iter k f (f x) = f (Nat.iter k f x).
+Proof.
+  induction k.
+  - reflexivity.
+  - simpl; congruence.
+Qed.
+
+Record loop_data (X : Type) : Type := {
+  measure : X -> nat;
+  step : X -> X;
+
+  step_measure : forall x, measure (step x) <= measure x
+  }.
+
+Arguments measure {_} _ _.
+Arguments step {_} _ _.
+
+Arguments step_measure {_} _ _.
+
+Fixpoint loop_aux {X} (l : loop_data X) (x : X)
+  (a : Acc (Wf_nat.ltof _ (measure l)) x) {struct a} : X.
+Proof.
+  destruct (le_lt_eq_dec _ _ (step_measure l x)).
+  - destruct a.
+    apply (loop_aux X l (step l x)).
+    apply H. exact l0.
+  - exact x.
+Defined.
+
+Fixpoint loop_aux_ext {X} (l : loop_data X) (x : X)
+  (a : Acc (Wf_nat.ltof _ (measure l)) x) {struct a} :
+  forall a',
+  loop_aux l x a = loop_aux l x a'.
+Proof.
+  destruct a, a'; simpl.
+  destruct le_lt_eq_dec.
+  - apply loop_aux_ext.
+  - reflexivity.
+Defined.
+
+Definition loop {X} (l : loop_data X) (x : X) : X :=
+  loop_aux l x (Wf_nat.well_founded_ltof X (measure l) x).
+
+Lemma loop_eq {X} (l : loop_data X) (x : X) :
+  loop l x =
+    match le_lt_eq_dec _ _ (step_measure l x) with
+    | left _ => loop l (step l x)
+    | right _ => x
+    end.
+Proof.
+  unfold loop at 1.
+  unfold loop_aux.
+  destruct (Wf_nat.well_founded_ltof X (measure l) x).
+  - destruct (le_lt_eq_dec).
+    + unfold loop.
+      unfold loop_aux.
+      apply loop_aux_ext.
+    + reflexivity.
+Defined.
+
+
+
+Lemma loop_measure_aux {X} (l : loop_data X) : forall n x, n = measure l x ->
+  measure l (loop l x) = measure l (step l (loop l x)).
+Proof.
+  intro n.
+  induction (Wf_nat.lt_wf n) as [n _ IHn].
+  intros.
+  rewrite loop_eq.
+  destruct le_lt_eq_dec.
+  - rewrite (IHn (measure l (step l x))); [reflexivity| |reflexivity].
+    rewrite H.
+    pose (step_measure l x). lia.
+  - symmetry; exact e.
+Qed.
+
+Lemma loop_measure {X} (l : loop_data X) : forall x,
+  measure l (loop l x) = measure l (step l (loop l x)).
+Proof.
+  intros.
+  eapply loop_measure_aux; reflexivity.
+Qed.
+
+Lemma loop_iter_aux {X} (l : loop_data X) : forall n x, n = measure l x ->
+  {n : nat & loop l x = Nat.iter n (step l) x}.
+Proof.
+  intro n.
+  induction (Wf_nat.lt_wf n) as [n _ IHn].
+  intros.
+  rewrite loop_eq.
+  destruct le_lt_eq_dec.
+  - assert (pf : measure l (step l x) < n).
+    { rewrite H.
+      pose proof (step_measure l x); lia.
+    }
+    destruct (IHn (measure l (step l x)) pf (step l x) eq_refl) as [k Hk].
+    exists (S k).
+    rewrite Hk.
+    simpl.
+    apply iter_lemma.
+  - exists 0; reflexivity.
+Defined.
+
+Lemma loop_iter {X} (l : loop_data X) : forall x,
+  {n : nat & loop l x = Nat.iter n (step l) x}.
+Proof.
+  intro x.
+  exact (loop_iter_aux l (measure l x) x eq_refl).
+Defined.
+
+Record validity_data {X} (l : loop_data X) : Type := {
+  valid : X -> Type;
+  step_valid : forall x, valid x -> valid (step l x)
+  }.
+
+Arguments valid {_} {_} _ _.
+Arguments step_valid {_} _ {_} _.
+
+Lemma iter_step_valid {X} (l : loop_data X) (v : validity_data l) :
+  forall n x, valid v x -> valid v (Nat.iter n (step l) x).
+Proof.
+  induction n; intros x x_v.
+  - exact x_v.
+  - simpl.
+    apply step_valid.
+    apply IHn.
+    exact x_v.
+Defined.
+
+Lemma loop_valid {X} (l : loop_data X) (v : validity_data l) : forall x,
+  valid v x -> valid v (loop l x).
+Proof.
+  intros.
+  destruct (loop_iter l x) as [n n_v].
+  rewrite n_v.
+  now apply iter_step_valid.
+Defined.
